Update Examples, pseudo and real identity

theories/Example.v
@@ -13,15 +13,19 @@ From Translation Require Import util Sorts SAst SLiftSubst SCommon ITyping
 Open Scope string_scope.
 Open Scope x_scope.
 
-(*! EXAMPLE 1 (NEW) *)
+(*! EXAMPLE 1 *)
 
-Fail Definition pseudoid := fun (A B : Type) (e : A = B) (x : A) => x : B.
+Fail Definition pseudoid (A B : Type) (e : A = B) (x : A) : B := x.
 
-(* Definition pseudoid (A B : Type) (e : A = B) (x : A) : B := {! x !}. *)
-Quote Definition pseudoid := (fun (A B : Type) (e : A = B) (x : A) => {! x !} : B).
+Definition pseudoid (A B : Type) (e : A = B) (x : A) : B := {! x !}.
+
+Quote Definition pseudoid_term := 
+  ltac:(let t := eval compute in pseudoid in exact t).
+Quote Definition pseudoid_type := 
+  ltac:(let T := type of pseudoid in exact T).
 
 Definition pretm_pseudoid :=
-  Eval lazy in fullquote (2 ^ 18) Σ [] pseudoid empty empty.
+  Eval lazy in fullquote (2 ^ 18) Σ [] pseudoid_term empty empty.
 Definition tm_pseudoid :=
   Eval lazy in 
   match pretm_pseudoid with
@@ -29,7 +33,6 @@ Definition tm_pseudoid :=
   | Error _ => sRel 0
   end.
 
-Quote Definition pseudoid_type := (forall (A B : Type) (e : A = B) (x : A), B).
 Definition prety_pseudoid :=
   Eval lazy in fullquote (2 ^ 18) Σ [] pseudoid_type empty empty.
 Definition ty_pseudoid :=
@@ -65,459 +68,70 @@ Make Definition coq_pseudoid :=
       in exact t
   ).
 
-(*! EXAMPLE 1:
-    λ A B e x ⇒ x : ∀ (A B : Type), A = B → A → B
-    It uses reflection to be well-typed.
-    It gets translated to
-    λ A B e x ⇒ transport e x : ∀ (A B : Type), A = B → A → B.
-*)
+(*! EXAMPLE 2 *)
 
-(* We begin with an ETT derivation *)
+Definition realid := fun (A B : Type) (x : A) => x.
+Quote Definition realid_term := 
+  ltac:(let t := eval compute in realid in exact t).
+Quote Definition realid_type := 
+  ltac:(let T := type of realid in exact T).
 
-Definition tyl :=
-  [ sSort tt ;
-    sSort tt ;
-    sEq (sSort tt) (sRel 1) (sRel 0) ;
-    sRel 2 ;
-    sRel 2
-  ].
+Definition pretm_realid :=
+  Eval lazy in fullquote (2 ^ 18) Σ [] realid_term empty empty.
+Definition tm_realid :=
+  Eval lazy in 
+  match pretm_realid with
+  | Success t => t
+  | Error _ => sRel 0
+  end.
 
-Definition ty : sterm := multiProd tyl.
+Definition prety_realid :=
+  Eval lazy in fullquote (2 ^ 18) Σ [] realid_type empty empty.
+Definition ty_realid :=
+  Eval lazy in 
+  match prety_realid with
+  | Success t => t
+  | Error _ => sRel 0
+  end.
 
-Definition tm : sterm := multiLam tyl (sRel 0).
-
-Fact tmty : Σi ;;; [] |-x tm : ty.
+Lemma type_realid : Σi ;;; [] |-x tm_realid : ty_realid.
 Proof.
-  eapply type_multiLam.
-  - constructor.
-  - econstructor.
-    + eapply type_Sort. constructor.
-    + econstructor.
-      * eapply type_Sort.
-        repeat econstructor.
-      * econstructor.
-        -- eapply type_Eq.
-           ++ repeat constructor.
-              ** repeat econstructor.
-           ++ refine (type_Rel _ _ _ _ _).
-              ** repeat econstructor.
-              ** cbn. omega.
-           ++ refine (type_Rel _ _ _ _ _).
-              ** repeat econstructor.
-              ** cbn. omega.
-        -- econstructor.
-           ++ refine (type_Rel _ _ _ _ _).
-              ** repeat econstructor.
-              ** cbn. omega.
-           ++ econstructor.
-              ** refine (type_Rel _ _ _ _ _).
-                 --- repeat econstructor.
-                 --- cbn. omega.
-              ** eapply type_conv''.
-                 --- refine (type_Rel _ _ _ _ _).
-                     +++ repeat econstructor.
-                     +++ cbn. omega.
-                 --- cbn. eapply reflection.
-                     instantiate (2 := sRel 1).
-                     refine (type_Rel _ _ _ _ _).
-                     +++ repeat econstructor.
-                     +++ cbn. omega.
-                 --- refine (type_Rel _ _ _ _ _).
-                     +++ repeat econstructor.
-                     +++ cbn. omega.
-  Unshelve.
-  all: cbn; omega.
-Defined.
-
-(* Then we translate this ETT derivation to get an ITT term *)
-
-Definition itt_tm : sterm.
-  destruct (type_translation tmty istrans_nil) as [A [t h]].
-  exact t.
-Defined.
-
-Definition itt_tm' := ltac:(let t := eval lazy in itt_tm in exact t).
-
-Definition tc_tm : tsl_result term :=
-  tsl_rec (2 ^ 18) Σ [] itt_tm'.
-
-Definition tc_tm' := ltac:(let t := eval lazy in tc_tm in exact t).
-
-Make Definition coq_tm :=
-  ltac:(
-    let t := eval lazy in
-             (match tc_tm' with
-              | Success _ t => t
-              | _ => tSort Universe.type0
-              end)
-      in exact t
-  ).
-
-(*! EXAMPLE 2:
-    λ A x ⇒ x : ∀ (A : Type), A → A
-    It gets translated to itself.
-*)
-
-Definition tyl0 :=
-  [ sSort tt ;
-    sRel 0 ;
-    sRel 1
-  ].
-
-Definition ty0 : sterm := multiProd tyl0.
-
-Definition tm0 : sterm := multiLam tyl0 (sRel 0).
-
-Lemma tmty0 : Σi ;;; [] |-x tm0 : ty0.
-Proof.
-  eapply type_multiLam.
-  - constructor.
-  - econstructor.
-    + repeat econstructor.
-    + econstructor.
-      * refine (type_Rel _ _ _ _ _).
-        -- repeat econstructor.
-        -- cbn. omega.
-      * econstructor.
-        -- refine (type_Rel _ _ _ _ _).
-           ++ repeat econstructor.
-           ++ cbn. omega.
-        -- refine (type_Rel _ _ _ _ _).
-           ++ repeat econstructor.
-           ++ cbn. omega.
-  Unshelve. all: cbn; omega.
-Defined.
-
-Definition itt_tm0 : sterm.
-  destruct (type_translation tmty0 istrans_nil) as [A [t [_ h]]].
-  exact t.
-Defined.
-
-Definition itt_tm0' := ltac:(let t := eval lazy in itt_tm0 in exact t).
-
-Definition tc_tm0 : tsl_result term :=
-  tsl_rec (2 ^ 18) Σ [] itt_tm0'.
-
-Definition tc_tm0' := ltac:(let t := eval lazy in tc_tm0 in exact t).
-
-Make Definition coq_tm0 :=
-  ltac:(
-    let t := eval lazy in
-             (match tc_tm0' with
-              | Success _ t => t
-              | _ => tSort Universe.type0
-              end)
-      in exact t
-  ).
-
-
-(*! EXAMPLE 3:
-    nat
-    It gets translated to itself.
-*)
-
-Lemma natty : Σi ;;; [] |-x sAx "nat" : sSort tt.
-Proof.
+  unfold tm_realid, ty_realid.
   ettcheck.
 Defined.
 
-Definition itt_nat : sterm.
-  destruct (type_translation natty istrans_nil) as [A [t [_ h]]].
-  exact t.
-Defined.
+Definition itt_realid : sterm :=
+  Eval lazy in
+  let '(_ ; t ; _) := type_translation type_realid istrans_nil in t.
 
-Definition itt_nat' := ltac:(let t := eval lazy in itt_nat in exact t).
+Definition tc_realid : tsl_result term :=
+  Eval lazy in
+  tsl_rec (2 ^ 18) Σ [] itt_realid empty.
 
-Definition tc_nat : tsl_result term :=
-  tsl_rec (2 ^ 18) Σ [] itt_nat'.
-
-Definition tc_nat' := ltac:(let t := eval lazy in tc_nat in exact t).
-
-Make Definition coq_nat :=
+Make Definition coq_realid :=
   ltac:(
     let t := eval lazy in
-             (match tc_nat' with
-              | Success _ t => t
-              | _ => tSort Universe.type0
+             (match tc_realid with
+              | FinalTranslation.Success _ t => t
+              | _ => tRel 0
               end)
       in exact t
   ).
 
-(*! EXAMPLE 3':
-    zero
-    It gets translated to itself.
-*)
+(*! EXAMPLE 3 *)
 
-Lemma zeroty : Σi ;;; [] |-x sAx "zero" : sAx "nat".
-Proof.
-  ettcheck.
-Defined.
+Fail Equations vrev {A n m} (v : vec A n) (acc : vec A m) : vec A (n + m) :=
+  vrev vnil acc := acc ;
+  vrev (vcons a n v) acc := vrev v (vcons a m acc).
 
-Definition itt_zero : sterm.
-  destruct (type_translation zeroty istrans_nil) as [A [t [_ h]]].
-  exact t.
-Defined.
+Equations vrev {A n m} (v : vec A n) (acc : vec A m) : vec A (n + m) :=
+  vrev vnil acc := acc ;
+  vrev (vcons a n v) acc := {! vrev v (vcons a m acc) !}.
 
-Definition itt_zero' := ltac:(let t := eval lazy in itt_zero in exact t).
-
-Definition tc_zero : tsl_result term :=
-  tsl_rec (2 ^ 18) Σ [] itt_zero'.
-
-Definition tc_zero' := ltac:(let t := eval lazy in tc_zero in exact t).
-
-Make Definition coq_zero :=
-  ltac:(
-    let t := eval lazy in
-             (match tc_zero' with
-              | Success _ t => t
-              | _ => tSort Universe.type0
-              end)
-      in exact t
-  ).
-
-(*! EXAMPLE 3'':
-    succ zero
-    It gets translated to itself.
-*)
-
-Definition sNat := sAx "nat".
-Definition sZero := sAx "zero".
-Definition sSucc n :=
-  sApp (sAx "succ") sNat sNat n.
-
-Lemma type_zero :
-  forall {Γ},
-    wf Σi Γ ->
-    Σi ;;; Γ |-x sZero : sNat.
-Proof.
-  unfold sZero, sNat.
-  intros Γ h.
-  ettcheck.
-Defined.
-
-Lemma type_succ :
-  forall {Γ n},
-    Σi ;;; Γ |-x n : sNat ->
-    Σi ;;; Γ |-x sSucc n : sNat.
-Proof.
-  unfold sSucc, sNat.
-  intros Γ n h.
-  pose proof (typing_wf h) as hw.
-  ettcheck. assumption.
-Defined.
-
-Definition sOne := sSucc sZero.
-
-Lemma onety : Σi ;;; [] |-x sOne : sNat.
-Proof.
-  unfold sOne. eapply type_succ. eapply type_zero. constructor.
-Defined.
-
-Definition itt_one : sterm.
-  destruct (type_translation onety istrans_nil) as [A [t [_ h]]].
-  exact t.
-Defined.
-
-Definition itt_one' := ltac:(let t := eval lazy in itt_one in exact t).
-
-Definition tc_one : tsl_result term :=
-  tsl_rec (2 ^ 18) Σ [] itt_one'.
-
-Definition tc_one' := ltac:(let t := eval lazy in tc_one in exact t).
-
-Make Definition coq_one :=
-  ltac:(
-    let t := eval lazy in
-             (match tc_one' with
-              | Success _ t => t
-              | _ => tSort Universe.type0
-              end)
-      in exact t
-  ).
-
-
-(* (*! EXAMPLE 4.1: *)
-(*     vcons one zero vnil *)
-(*     It gets translated to itself (but checking takes a long time!). *)
-(* *) *)
-
-(* Open Scope type_scope. *)
-
-(* Definition sVec A n := *)
-(*   Apps (sAx "vec") [ (nNamed "A", sSort tt) ; (nAnon, sNat) ] (sSort tt) [ A ; n ]. *)
-
-(* Definition sVnil A := *)
-(*   sApp (sAx "vnil") *)
-(*        (sSort tt) *)
-(*        (sVec (sRel 0) sZero) *)
-(*        A. *)
-
-(* Definition sVcons A a n v := *)
-(*   Apps *)
-(*     (sAx "vcons") *)
-(*     [ (nNamed "A", sSort tt) ; *)
-(*       (nAnon, sRel 0) ; *)
-(*       (nNamed "n", sNat) ; *)
-(*       (nAnon, sVec (sRel 2) (sRel 0)) *)
-(*     ] *)
-(*     (sVec (sRel 3) (sSucc (sRel 1))) *)
-(*     [ A ; a ; n ; v ]. *)
-
-(* Lemma type_vec : *)
-(*   forall {Γ A n}, *)
-(*     Σi ;;; Γ |-x A : sSort tt -> *)
-(*     Σi ;;; Γ |-x n : sNat -> *)
-(*     Σi ;;; Γ |-x sVec A n : sSort tt. *)
-(* Proof. *)
-(*   unfold sVcons, sVec, sVnil, sOne, sSucc, sNat, sZero. *)
-(*   intros Γ A n hA hn. *)
-(*   pose proof (typing_wf hA) as hw. *)
-(*   simpl. ettcheck. all: assumption. *)
-(* Defined. *)
-
-(* Lemma type_vnil : *)
-(*   forall {Γ A}, *)
-(*     Σi ;;; Γ |-x A : sSort tt -> *)
-(*     Σi ;;; Γ |-x sVnil A : sVec A sZero. *)
-(* Proof. *)
-(*   unfold sVcons, sVec, sVnil, sSucc, sNat, sZero. *)
-(*   intros Γ A h. simpl. *)
-(*   pose proof (typing_wf h) as hw. *)
-(*   Opaque lift. *)
-(*   ettcheck. all: try assumption. *)
-(*   - unfold sVec, sNat. simpl. ettcheck. *)
-(*   - simpl. rewrite lift00. constructor. *)
-(*     ettcheck. assumption. *)
-(* Defined. *)
-
-(* Transparent lift. *)
-
-(* (* Lemma type_vcons : *) *)
-(* (*   forall {Γ A a n v}, *) *)
-(* (*     Σi ;;; Γ |-x A : sSort 0 -> *) *)
-(* (*     Σi ;;; Γ |-x a : A -> *) *)
-(* (*     Σi ;;; Γ |-x n : sNat -> *) *)
-(* (*     Σi ;;; Γ |-x v : sVec A n -> *) *)
-(* (*     Σi ;;; Γ |-x sVcons A a n v : sVec A (sSucc n). *) *)
-(* (* Proof. *) *)
-(* (*   unfold sVcons, sVec, sVnil, sSucc, sNat, sZero. *) *)
-(* (*   intros Γ A a n v hA ha hn hv. *) *)
-(* (*   pose proof (typing_wf ha) as hw. *) *)
-(* (*   simpl. *) *)
-(* (*   ettcheck. *) *)
-(* (*   all: rewrite ?lift00. all: try eassumption. *) *)
-(* (*   - *) *)
-
-(* Definition vtest := sVcons sNat sOne sZero (sVnil sNat). *)
-
-(* Lemma vtestty : Σi ;;; [] |-x vtest : sVec sNat sOne. *)
-(* Proof. *)
-(*   unfold vtest, sVcons, sVec, sVnil, sOne, sSucc, sNat, sZero. lazy. *)
-(*   ettcheck. *)
-(* Defined. *)
-
-(* Definition itt_vtest : sterm. *)
-(*   destruct (type_translation vtestty istrans_nil) as [A [t [_ h]]]. *)
-(*   exact t. *)
-(* Defined. *)
-
-(* Definition itt_vtest' := ltac:(let t := eval lazy in itt_vtest in exact t). *)
-
-(* Definition tc_vtest : tsl_result term := *)
-(*   tsl_rec (2 ^ 18) Σ [] itt_vtest'. *)
-
-(* Definition tc_vtest' := ltac:(let t := eval lazy in tc_vtest in exact t). *)
-
-(* Make Definition coq_vtest := *)
-(*   ltac:( *)
-(*     let t := eval lazy in *)
-(*              (match tc_vtest' with *)
-(*               | Success t => t *)
-(*               | _ => tSort Universe.type0 *)
-(*               end) *)
-(*       in exact t *)
-(*   ). *)
-
-
-(* (*! EXAMPLE 4.2: *)
-(*     plus *)
-(* *) *)
-(* Definition snatrec P Pz Ps n := *)
-(*   Apps *)
-(*     (sAx "nat_rect") *)
-(*     [ (nNamed "P", sNat ==> sSort 0) ; *)
-(*       (nAnon, sApp (sRel 0) sNat (sSort 0) sZero) ; *)
-(*       (nAnon, sProd (nNamed "n") sNat (sApp (sRel 2) sNat (sSort 0) (sRel 0) ==> sApp (sRel 2) sNat (sSort 0) (sSucc (sRel 0)))) ; *)
-(*       (nNamed "n", sNat) *)
-(*     ] *)
-(*     (sApp (sRel 3) sNat (sSort 0) (sRel 0)) *)
-(*     [ P ; Pz ; Ps ; n ]. *)
-
-(* Definition plus n m := *)
-(*   snatrec (sLambda (nNamed "n") sNat (sSort 0) sNat) *)
-(*           m *)
-(*           (multiLam [ sNat ; sNat ; sNat ] (sSucc (sRel 0))) *)
-(*           n. *)
-
-(* Definition cplus := *)
-(*   sLambda (nNamed "n") sNat (sNat ==> sNat) *)
-(*   (sLambda (nNamed "m") sNat sNat (plus (sRel 1) (sRel 0))). *)
-
-(* Ltac ettcong := *)
-(*   lazymatch goal with *)
-(*   | |- ?Σ ;;; ?Γ |-x ?t = _ : ?T => *)
-(*     lazymatch t with *)
-(*     | sRel ?n => eapply eq_reflexivity *)
-(*     | sSort _ => eapply eq_reflexivity *)
-(*     | sProd _ _ _ => eapply cong_Prod *)
-(*     | sLambda _ _ _ _ => eapply cong_Lambda *)
-(*     | sApp _ _ _ _ => eapply cong_App *)
-(*     | sSum _ _ _ => eapply cong_Sum *)
-(*     | sPair _ _ _ _ => eapply cong_Pair *)
-(*     | sPi1 _ _ _ => eapply cong_Pi1 *)
-(*     | sPi2 _ _ _ => eapply cong_Pi2 *)
-(*     | sEq _ _ _ => eapply cong_Eq *)
-(*     | sRefl _ _ => eapply cong_Refl *)
-(*     | sAx _ => eapply eq_reflexivity *)
-(*     | _ => fail "No congruence rule for" t *)
-(*     end *)
-(*   | _ => fail "Not applicable" *)
-(*   end. *)
-
-(* Lemma xmeta_eq_conv : *)
-(*   forall {Σ Γ A B T U}, *)
-(*     Σ ;;; Γ |-x A = B : U -> *)
-(*     T = U -> *)
-(*     Σ ;;; Γ |-x A = B : T. *)
-(* Proof. *)
-(*   intros Σ Γ A B T U h e. destruct e. assumption. *)
-(* Defined. *)
-
-(* Ltac ettconvcheck1 := *)
-(*   lazymatch goal with *)
-(*   | |- ?Σ ;;; ?Γ |-x ?t = ?u : ?T => *)
-(*     first [ *)
-(*       eapply xmeta_eq_conv ; [ ettcong | lazy ; reflexivity ] *)
-(*     | eapply eq_conv ; [ ettcong | .. ] *)
-(*     (* | eapply meta_ctx_conv ; [ *) *)
-(*     (*     eapply meta_conv ; [ ettintro | lazy ; try reflexivity ] *) *)
-(*     (*   | cbn ; try reflexivity *) *)
-(*     (*   ] *) *)
-(*     ] *)
-(*   | |- wf ?Σ ?Γ => first [ assumption | econstructor ] *)
-(*   | |- sSort _ = sSort _ => first [ lazy ; reflexivity | shelve ] *)
-(*   | |- type_glob _ => first [ assumption | glob ] *)
-(*   | _ => fail "Not applicable" *)
-(*   end. *)
-
-(* Lemma plusty : Σi ;;; [] |-x cplus : sNat ==> sNat ==> sNat. *)
-(* Proof. *)
-(*   unfold cplus, plus, snatrec, sZero, sSucc, sNat, Arrow. simpl. *)
-(*   (* ettcheck. *) *)
-(*   (* - cbn. repeat ettconvcheck1. all: ettcheck. *) *)
-(* Abort. *)
-
-(* (*! EXAMPLE 4.? (more ambitious): *)
-(*     rev A n m (v : vec A n) (acc : vec A m) : vec A (n + m) := *)
-(*       vec_rect A ??? *)
-(* *) *)
+(* TODO
+   - We need to tell equations to yield a definition with eliminators instead.
+   - Extend the context with what is needed for this to type check:
+     - nat(O,S), vec(vnil, vcons, vec_rect)
+     - vec A (0 + m) = vec A m
+     - vec A (n + S m) = vec A (S n + m)
+ *)
